theories/tactics/utp_alpha_tac.thy
@@ -7,7 +7,8 @@
 header {* Proof Tactic for Alphabetised Predicates *}
 
 theory utp_alpha_tac
-imports "../alpha/utp_alpha_pred"
+imports 
+  "../alpha/utp_alpha_pred"
 begin
 
 text {* Theorem Attribute *}
@@ -46,107 +47,75 @@ subsection {* Distribution Theorems *}
 theorem EvalA_LiftA [evala] :
 "f \<in> WF_BINDING_PRED \<langle>a\<rangle>\<^sub>f \<Longrightarrow>
  \<lbrakk>LiftA a f\<rbrakk>\<pi> = LiftP f"
-apply (simp add: EvalA_def)
-apply (simp add: LiftA_rep_eq)
-done
+  by (simp add: EvalA_def LiftA_rep_eq)
 
 theorem EvalA_EqualsA [evala] :
-"\<lbrakk>v =\<alpha> x\<rbrakk>\<pi> = (v =p x)"
-apply (simp add: EvalA_def)
-apply (simp add: EqualsA.rep_eq)
-done
+"\<lbrakk>v =\<^sub>\<alpha> x\<rbrakk>\<pi> = (v =\<^sub>p x)"
+  by (simp add: EvalA_def EqualsA.rep_eq)
 
 theorem EvalA_TrueA [evala] :
-"\<lbrakk>true a\<rbrakk>\<pi> = true"
-apply (simp add: EvalA_def)
-apply (simp add: TrueA_rep_eq)
-done
+"\<lbrakk>true\<^bsub>a\<^esub>\<rbrakk>\<pi> = true"
+  by (simp add: EvalA_def TrueA_rep_eq)
 
 theorem EvalA_FalseA [evala] :
-"\<lbrakk>false a\<rbrakk>\<pi> = false"
-apply (simp add: EvalA_def)
-apply (simp add: FalseA_rep_eq)
-done
+"\<lbrakk>false\<^bsub>a\<^esub>\<rbrakk>\<pi> = false"
+  by (simp add: EvalA_def FalseA_rep_eq)
 
 theorem EvalA_ExtA [evala] :
-"\<lbrakk>p \<oplus>\<alpha> a\<rbrakk>\<pi> = \<lbrakk>p\<rbrakk>\<pi>"
-apply (simp add: EvalA_def)
-apply (simp add: ExtA.rep_eq)
-done
+"\<lbrakk>p \<oplus>\<^sub>\<alpha> a\<rbrakk>\<pi> = \<lbrakk>p\<rbrakk>\<pi>"
+  by (simp add: EvalA_def ExtA.rep_eq)
 
 theorem EvalA_ResA [evala] :
-"\<lbrakk>p \<ominus>\<alpha> a\<rbrakk>\<pi> = (\<exists>p \<langle>a\<rangle>\<^sub>f . \<lbrakk>p\<rbrakk>\<pi>)"
-apply (simp add: EvalA_def)
-apply (simp add: ResA.rep_eq)
-done
+"\<lbrakk>p \<ominus>\<^sub>\<alpha> a\<rbrakk>\<pi> = (\<exists>\<^sub>p \<langle>a\<rangle>\<^sub>f . \<lbrakk>p\<rbrakk>\<pi>)"
+  by (simp add: EvalA_def ResA.rep_eq)
 
 theorem EvalA_NotA [evala] :
-"\<lbrakk>\<not>\<alpha> p\<rbrakk>\<pi> = \<not>p \<lbrakk>p\<rbrakk>\<pi>"
-apply (simp add: EvalA_def)
-apply (simp add: NotA.rep_eq)
-done
+"\<lbrakk>\<not>\<^sub>\<alpha> p\<rbrakk>\<pi> = \<not>\<^sub>p \<lbrakk>p\<rbrakk>\<pi>"
+  by (simp add: EvalA_def NotA.rep_eq)
 
 theorem EvalA_AndA [evala] :
-"\<lbrakk>p1 \<and>\<alpha> p2\<rbrakk>\<pi> = \<lbrakk>p1\<rbrakk>\<pi> \<and>p \<lbrakk>p2\<rbrakk>\<pi>"
-apply (simp add: EvalA_def)
-apply (simp add: AndA.rep_eq)
-done
+"\<lbrakk>p1 \<and>\<^sub>\<alpha> p2\<rbrakk>\<pi> = \<lbrakk>p1\<rbrakk>\<pi> \<and>\<^sub>p \<lbrakk>p2\<rbrakk>\<pi>"
+  by (simp add: EvalA_def AndA.rep_eq)
 
 theorem EvalA_OrA [evala] :
-"\<lbrakk>p1 \<or>\<alpha> p2\<rbrakk>\<pi> = \<lbrakk>p1\<rbrakk>\<pi> \<or>p \<lbrakk>p2\<rbrakk>\<pi>"
-apply (simp add: EvalA_def)
-apply (simp add: OrA.rep_eq)
-done
+"\<lbrakk>p1 \<or>\<^sub>\<alpha> p2\<rbrakk>\<pi> = \<lbrakk>p1\<rbrakk>\<pi> \<or>\<^sub>p \<lbrakk>p2\<rbrakk>\<pi>"
+  by (simp add: EvalA_def OrA.rep_eq)
 
 theorem EvalA_ImpliesA [evala] :
-"\<lbrakk>p1 \<Rightarrow>\<alpha> p2\<rbrakk>\<pi> = \<lbrakk>p1\<rbrakk>\<pi> \<Rightarrow>p \<lbrakk>p2\<rbrakk>\<pi>"
-apply (simp add: EvalA_def)
-apply (simp add: ImpliesA.rep_eq)
-done
+"\<lbrakk>p1 \<Rightarrow>\<^sub>\<alpha> p2\<rbrakk>\<pi> = \<lbrakk>p1\<rbrakk>\<pi> \<Rightarrow>\<^sub>p \<lbrakk>p2\<rbrakk>\<pi>"
+  by (simp add: EvalA_def ImpliesA.rep_eq)
 
 theorem EvalA_IffA [evala] :
-"\<lbrakk>p1 \<Leftrightarrow>\<alpha> p2\<rbrakk>\<pi> = \<lbrakk>p1\<rbrakk>\<pi> \<Leftrightarrow>p \<lbrakk>p2\<rbrakk>\<pi>"
-apply (simp add: EvalA_def)
-apply (simp add: IffA.rep_eq)
-done
+"\<lbrakk>p1 \<Leftrightarrow>\<^sub>\<alpha> p2\<rbrakk>\<pi> = \<lbrakk>p1\<rbrakk>\<pi> \<Leftrightarrow>\<^sub>p \<lbrakk>p2\<rbrakk>\<pi>"
+  by (simp add: EvalA_def IffA.rep_eq)
 
 theorem EvalA_ExistsA [evala] :
-"\<lbrakk>\<exists>\<alpha> a . p\<rbrakk>\<pi> = (\<exists>p \<langle>a\<rangle>\<^sub>f . \<lbrakk>p\<rbrakk>\<pi>)"
+"\<lbrakk>\<exists>\<^sub>\<alpha> a . p\<rbrakk>\<pi> = (\<exists>\<^sub>p \<langle>a\<rangle>\<^sub>f . \<lbrakk>p\<rbrakk>\<pi>)"
   by (simp add: EvalA_def ExistsA.rep_eq)
 
 theorem EvalA_ForallA [evala] :
-"\<lbrakk>\<forall>\<alpha> a . p\<rbrakk>\<pi> = (\<forall>p \<langle>a\<rangle>\<^sub>f . \<lbrakk>p\<rbrakk>\<pi>)"
+"\<lbrakk>\<forall>\<^sub>\<alpha> a . p\<rbrakk>\<pi> = (\<forall>\<^sub>p \<langle>a\<rangle>\<^sub>f . \<lbrakk>p\<rbrakk>\<pi>)"
   by (simp add: EvalA_def ForallA.rep_eq)
 
 theorem EvalA_ExistsResA [evala] :
-"\<lbrakk>\<exists>-\<alpha> a . p\<rbrakk>\<pi> = \<lbrakk>\<exists>\<alpha> a . p\<rbrakk>\<pi>"
-apply (simp add: EvalA_def)
-apply (simp add: ExistsResA.rep_eq)
-apply (simp add: ExistsA.rep_eq)
-done
+"\<lbrakk>\<exists>-\<^sub>\<alpha> a . p\<rbrakk>\<pi> = \<lbrakk>\<exists>\<^sub>\<alpha> a . p\<rbrakk>\<pi>"
+  by (simp add: EvalA_def ExistsResA.rep_eq ExistsA.rep_eq)
 
 theorem EvalA_ForallResA [evala] :
-"\<lbrakk>\<forall>-\<alpha> a . p\<rbrakk>\<pi> = \<lbrakk>\<forall>\<alpha> a . p\<rbrakk>\<pi>"
-apply (simp add: EvalA_def)
-apply (simp add: ForallResA.rep_eq)
-apply (simp add: ForallA.rep_eq)
-done
+"\<lbrakk>\<forall>-\<^sub>\<alpha> a . p\<rbrakk>\<pi> = \<lbrakk>\<forall>\<^sub>\<alpha> a . p\<rbrakk>\<pi>"
+  by (simp add: EvalA_def ForallResA.rep_eq ForallA.rep_eq)
 
 theorem EvalA_ClosureA [evala] :
-"\<lbrakk>[p]\<alpha>\<rbrakk>\<pi> = [\<lbrakk>p\<rbrakk>\<pi>]p"
-apply (simp add: EvalA_def)
-apply (simp add: ClosureA.rep_eq)
-done
+"\<lbrakk>[p]\<^sub>\<alpha>\<rbrakk>\<pi> = [\<lbrakk>p\<rbrakk>\<pi>]\<^sub>p"
+  by (simp add: EvalA_def ClosureA.rep_eq)
 
 theorem EvalA_RefA [evala] :
-"\<lbrakk>p1 \<sqsubseteq>\<alpha> p2\<rbrakk>\<pi> = \<lbrakk>p1\<rbrakk>\<pi> \<sqsubseteq>p \<lbrakk>p2\<rbrakk>\<pi>"
-apply (simp add: EvalA_def)
-apply (simp add: RefA.rep_eq)
-done
+"\<lbrakk>p1 \<sqsubseteq>\<^sub>\<alpha> p2\<rbrakk>\<pi> = \<lbrakk>p1\<rbrakk>\<pi> \<sqsubseteq>\<^sub>p \<lbrakk>p2\<rbrakk>\<pi>"
+  by (simp add: EvalA_def RefA.rep_eq)
 
 theorem EvalA_RenameA [evala] :
-"\<lbrakk>p[ss]\<alpha>\<rbrakk>\<pi> = \<lbrakk>p\<rbrakk>\<pi>[ss]"
-  by (simp add:EvalA_def RenameA.rep_eq)
+"\<lbrakk>ss\<bullet>p\<rbrakk>\<pi> = ss\<bullet>\<lbrakk>p\<rbrakk>\<pi>"
+  by (simp add:EvalA_def PermA.rep_eq)
 
 declare TautologyA_def [evala]
 declare ContradictionA_def [evala]
@@ -169,7 +138,10 @@ ML {*
       addsimps (evala.get ctxt)
       addsimps (closure.get ctxt)
       (* Closure alone seems not enough e.g. to simplify (p1 \<or>\<alpha> p2) \<sqsubseteq> p2. *)
-      addsimps (alphabet.get ctxt);
+      addsimps (alphabet.get ctxt)
+      addsimps (typing.get ctxt)
+      addsimps @{thms alphabet_simps}
+      addsimps @{thms alphabet_dist};
 *}
 
 ML {*
@@ -229,17 +201,11 @@ ML {* utp_alpha_tac2 *}
 subsection {* Proof Experiments *}
 
 theorem EvalA_test :
-"\<not>\<alpha> (\<not>\<alpha> p) = p"
-  by (utp_alpha_tac2)
-
-(*
-apply (utp_alpha_tac)
-apply (utp_pred_auto_tac)
-done
-*)
+"\<not>\<^sub>\<alpha> (\<not>\<^sub>\<alpha> p) = p"
+  by (utp_alpha_tac)
 
 theorem EvalA_contr:
-"p \<Rightarrow>\<alpha> false (\<alpha> p) = \<not>\<alpha> p"
+"p \<Rightarrow>\<^sub>\<alpha> false\<^bsub>\<alpha> p\<^esub> = \<not>\<^sub>\<alpha> p"
   by (utp_alpha_tac)
 
 end
